Flapjack/Tests.lean
@@ -7,6 +7,7 @@ import Flapjack.Test.Calls
 import Flapjack.Test.Loops
 import Flapjack.Test.Primitive
 import Flapjack.Test.Allocator
+import Flapjack.Test.AllocatorFunction
 import Flapjack.Test.WordToStack
 import Flapjack.RiscV.Correctness
 import Flapjack.RiscV.CorrectnessFfi
